Picinae_riscv.v
@@ -35,13 +35,14 @@
 Require Export Picinae_core.
 Require Export Picinae_theory.
 Require Export Picinae_statics.
+Require Export Picinae_auto.
 Require Export Picinae_finterp.
 Require Export Picinae_simplifier_v1_1.
 Require Export Picinae_ISA.
-Require Import NArith.
-Require Import ZArith.
-Require Import Program.Equality.
-Require Import Structures.Equalities.
+From Stdlib Require Import NArith.
+From Stdlib Require Import ZArith.
+From Stdlib Require Import Program.Equality.
+From Stdlib Require Import Structures.Equalities.
 Open Scope N.
 
 (* Variables found in IL code lifted from RISC-V native code: *)
@@ -102,6 +103,8 @@ Module Theory_RISCV := PicinaeTheory IL_RISCV.
 Export Theory_RISCV.
 Module Statics_RISCV := PicinaeStatics IL_RISCV Theory_RISCV.
 Export Statics_RISCV.
+Module Auto_RISCV := PicinaeAuto IL_RISCV Theory_RISCV Statics_RISCV.
+Export Auto_RISCV.
 Module FInterp_RISCV := PicinaeFInterp IL_RISCV Theory_RISCV Statics_RISCV.
 Export FInterp_RISCV.
 Module PSimpl_RISCV := Picinae_Simplifier_Base IL_RISCV.
@@ -244,7 +247,7 @@ Definition rv_decode_binop f :=
   end.
 
 Definition rv_decode_branch f :=
-  match f with 
+  match f with
   | 0 => R5_Beq | 1 => R5_Bne | 4 => R5_Blt | 5 => R5_Bge | 6 => R5_Bltu | 7 => R5_Bgeu
   | _ => (fun _ _ _ => R5_InvalidI)
   end.
